Fresh.dfy
@@ -1,0 +1,125 @@
+include "Util.dfy"
+include "Definitions.dfy"
+
+class Fresh {
+	/*
+	 * map of original variable to a fresh variable.
+	 * for example: vr <--> ivr or vr <--> fvr
+	 */
+	var m : map<Variable, set<Variable>>;
+	ghost var range : set<Variable>;	// fresh variables (range of map)
+	ghost var rotten : set<Variable>;	// non-fresh variables
+
+	constructor ()
+	modifies this
+	ensures Valid()
+	ensures |m| == 0 && range == {} && rotten == {}
+	{
+		m := map[];
+		range := {};
+		rotten := {};
+	}
+
+	predicate Valid() 
+	reads this
+	{
+		(|m| == 0 && range == {} && rotten == {}) || (
+		   (forall v :: v in m ==> v !in range)
+		&& (forall v :: v in range ==> v !in m)
+		&& (forall v :: v in rotten <==> v !in range)
+		&& (forall v :: v in range ==> v !in rotten)
+		&& (forall v :: v in m ==> m[v] <= range))
+	}
+
+	/*
+	 * in: V - subset of variables to which fresh names are required (V<=SV)
+	 * in: SV - set of all variables. Fresh variables should not exist in SV
+	 * out: fV - set of fresh variables, one per variable in V (fV !! SV)
+	 * side-effect: m is updated accordingly
+	 */
+	method {:verify true} CreateFresh(V: seq<Variable>, SV: seq<Variable>) returns (fV: seq<Variable>)
+	modifies this
+	requires Valid()
+	requires setOf(V) <= setOf(SV)
+	requires forall v :: v in V ==> v !in range
+	ensures Valid()
+	ensures setOf(fV) <= range
+	ensures setOf(fV) !! rotten
+	ensures setOf(fV) !! setOf(V)
+	ensures forall v :: v in fV ==> v !in SV
+	ensures forall v :: v in SV ==> v !in fV
+	ensures setOf(fV) !! setOf(SV)
+	ensures |fV| == |V|
+	{
+		var r := V;
+		var fV' : seq<Variable> := [];
+		while (r != [])
+		invariant forall v :: v in r ==> v in V
+		invariant forall v :: v in m ==> v in V
+		invariant forall v :: v in fV' ==> v !in m
+		decreases r
+		{
+			var name := freshName(r[0], SV, 0, {}, SV);
+			if (r[0] in m) {
+				m := m[r[0] := m[r[0]]+{name}]; // update 
+			} else {
+				m := m[r[0] := {name}]; // new map entry
+			}
+			assert name !in m;
+			fV' := fV' + [name];
+			assert name in fV';
+			r := r[1..];
+		}
+		
+		range := range + setOf(fV');
+		rotten := rotten + setOf(SV);
+		fV := fV';
+	}
+	
+	function method ComposeName(v: Variable, i : nat) : (res: Variable)
+	ensures res == v + intToString(i)
+	{
+		v + intToString(i)
+	}
+
+	lemma failedAttemptsBuildupLemma(v : Variable, 
+						 i : nat, 
+						 failedAttempts : set<Variable>)
+	ensures ComposeName(v, i) !in failedAttempts
+
+	method {:verify true} freshName(v : Variable, 
+					 SV: seq<Variable>, 
+					 i : nat, 
+					 failedAttempts : set<Variable>, 
+					 ghost SVorig : seq<Variable> ) 
+	returns (fv: Variable)
+	decreases |SV|
+	requires v in SV
+	requires SV <= SVorig
+	requires setOf(SV) !! failedAttempts
+	requires setOf(SV)+failedAttempts == setOf(SVorig)
+	requires forall j :: i > j >= 0 ==> ComposeName(v, j) in failedAttempts
+	requires ComposeName(v, i) !in failedAttempts
+	ensures fv !in SVorig
+	ensures fv != v
+	{
+		fv := ComposeName(v, i);
+		assert fv !in failedAttempts;
+		if (fv in SV) {
+			var i', SV', failedAttempts' := i+1, seqSubtraction(SV,[fv]), failedAttempts+{fv};
+			assert SV' < SV by {
+				assert fv !in SV' && fv in SV;
+				assume SV' <= SV;
+			}
+			assert ComposeName(v, i') !in failedAttempts' by
+			{ failedAttemptsBuildupLemma(v, i', failedAttempts');}
+			fv := freshName(v, SV', i', failedAttempts', SVorig);
+			assert fv !in SVorig;
+		}
+		else
+		{
+			assert fv !in SVorig;
+		}
+	}
+}
+/* end of class Fresh */
