Sliding-11.3.dfy
@@ -1,0 +1,83 @@
+include "Sliding-11.1-11.2.dfy"
+
+// Ch 11.3, Transformation 11.2
+method {:verify true} Sliding_PenlessCoSlice(
+	S: Statement, 
+	Vr: seq<Variable>, 
+	Vnr: seq<Variable>) 
+returns (result: Statement, Sv: Statement, Scov: Statement)
+requires Valid(S)
+requires setOf(Vr) !! setOf(Vnr) // TODO: fix
+ensures Valid(result)
+ensures Refinement(S, result)
+{
+	var freshV := new Fresh();
+
+	var Vr' := seqConjunction(Vr, fSetToSeq(def(S)));//Vr*def(S); 
+	var Vnr' := seqConjunction(Vnr, fSetToSeq(def(S)));//Vnr*def(S);
+	var coV := seqSubtraction(fSetToSeq(def(S)),(Vr'+Vnr'));//def(S)-(Vr'+Vnr')
+
+	Sv := ComputeSlice(S, setOf(Vr'+Vnr'));
+	Scov := ComputePenlessCoSlice(S, Vr'+Vnr', Vr');
+
+	var Vnr1 := seqConjunction(Vnr',fSetToSeq(input(Scov)));//Vnr'*input(Scov)
+	var Vnr2 := seqConjunction(Vnr',fSetToSeq(def(Scov)-input(Scov)));//Vnr'*(def(Scov)-input(Scov))
+	var coV11 := seqConjunction(coV,fSetToSeq(def(Sv)*input(Scov)));//coV*def(Sv)*input(Scov)
+
+	var iVr := freshV.CreateFresh(Vr', Vr+Vnr+fSetToSeq(glob(S)));
+	var iVnr := freshV.CreateFresh(Vnr', Vr+Vnr+fSetToSeq(glob(S)));
+	var icoV := freshV.CreateFresh(coV, Vr+Vnr+fSetToSeq(glob(S)));
+	var fVnr := freshV.CreateFresh(Vnr', Vr+Vnr+fSetToSeq(glob(S)));
+
+	
+	var iVnr1 := freshV.CreateFresh(Vnr1, Vr+Vnr+fSetToSeq(glob(S)));
+	var icoV11 := freshV.CreateFresh(coV11, Vr+Vnr+fSetToSeq(glob(S)));
+	var fVnr1 := freshV.CreateFresh(Vnr1, Vr+Vnr+fSetToSeq(glob(S)));
+	var fVnr2 := freshV.CreateFresh(Vnr2, Vr+Vnr+fSetToSeq(glob(S)));
+
+	// Provided... TODO: "requires"
+	var fVr := freshV.CreateFresh(Vr', Vr+Vnr+fSetToSeq(glob(S)));
+	var Scov' := ComputeCoSlice(S, Vr'+Vnr', Vr', fVr);
+	assert setOf(Vr') !! glob(Scov');
+
+	var decl : seq<Variable> := iVnr1+icoV11+fVnr1+fVnr2;
+	var ivars : seq<Variable> := iVnr1+icoV11;
+	var vars : seq<Variable> := Vnr1+coV11;
+	var vnrs : seq<Variable> := Vnr1+Vnr2;
+	var fvars : seq<Variable> := fVnr1+fVnr2;
+
+	var varse := seqVarToSeqExpr(vars);
+	var vnrse := seqVarToSeqExpr(vnrs);
+	var ivarse := seqVarToSeqExpr(ivars);
+	var fvarse := seqVarToSeqExpr(fvars);
+	var S' := SeqComp(Assignment(ivars, varse),
+				 SeqComp(Sv, 
+				  SeqComp(Assignment(fvars, vnrse),
+				   SeqComp(Assignment(vars, ivarse),
+				    SeqComp(Scov, Assignment(vnrs, fvarse))))));
+	result := LocalDeclaration(decl,S');
+	assert Valid(result); // <--- result is NOT valid. Why?
+	
+	var S'' := Live(Vr'+Vnr'+coV,S');
+//	assert Refinement(S, S'');
+//   forall P: Predicate,s: State :: (wp(S1,P).0.requires(s) && wp(S2,P).0.requires(s) && wp(S1,P).0(s) ==> wp(S2,P).0(s))
+
+	forall P: Predicate,s: State {
+		calc {
+			wp(S,P).0(s);
+			==> {Refinement11_1(S, Sv, Scov,
+								Vr', 
+								Vnr', 
+								coV,
+								iVr,
+								iVnr,
+								icoV,
+								fVr,
+								fVnr);
+			}
+			wp(S'',P).0(s);
+			== {}
+			wp(result,P).0(s);
+		}
+	}
+}
