Sliding-8-9-10.dfy
@@ -1,0 +1,90 @@
+include "FinalUseSubstitution.dfy"
+include "SliceRefinements.dfy"
+include "Fresh.dfy"
+
+//include "SSA.dfy"
+/* TODO:
+ * Prove SliceRefinement
+ * Prove CoSliceRefinement
+ * Prove Refinement by above + Corollary5_4_Lemma
+ */
+// Ch. 8 Fig 8.1
+function method {:verify true} ComputeSlides(S: Statement, V: seq<Variable>) : (S': Statement)
+reads *
+requires Valid(S)
+ensures Valid(S')
+{
+	if setOf(V)*def(S) == {} then Skip
+	else
+	match S {
+		case Skip => Skip
+		case Assignment(LHS, RHS) => GetAssignmentsOfV(LHS, RHS, V)
+		case SeqComp(S1, S2) => SeqComp(ComputeSlides(S1,V), ComputeSlides(S2,V))
+		case IF(B0, Sthen, Selse) => IF(B0, ComputeSlides(Sthen, V), ComputeSlides(Selse, V))
+		case DO(B, S) => DO(B, ComputeSlides(S, V))
+		case LocalDeclaration(L, S0) => ComputeSlides(S0, V)
+		case Live(L, S0) => ComputeSlides(S0, V)
+	}
+}
+
+// Ch. 9 Fig 9.1
+function method {:verify true} ComputeSlidesDepRtc(S: Statement, V: set<Variable>) 
+	: (V': set<Variable>)
+reads *
+requires Valid(S)
+ensures V <= V'
+decreases glob(S)-V
+{
+	var slidesSv := ComputeSlides(S, fSetToSeq(V));
+	var U := glob(slidesSv)*def(S);
+
+	if U <= V then V else ComputeSlidesDepRtc(S, V+U)
+}
+
+// Ch. 9 Fig 9.1
+method {:verify true} ComputeSlice(S: Statement, V: set<Variable>) 
+returns (Sv: Statement)
+requires Valid(S) 
+//ensures Refinement(Live(fSetToSeq(V), S), Live(fSetToSeq(V), Sv))
+ensures def(Sv)<=def(S)
+ensures glob(Sv)<=glob(S)
+ensures Valid(Sv)
+{
+	var Vstar := ComputeSlidesDepRtc(S, V);
+	Sv := ComputeSlides(S, fSetToSeq(Vstar));
+	assert Valid(Sv);
+	assert def(Sv)<=def(S) by {defOfPratialSPartialToDefSLemma(S, Sv);}
+	assert glob(Sv)<=glob(S) by {globOfPartialSPartialToGlobSLemma(S, Sv);}
+}
+
+// Ch. 10 Fig 10.2
+method {:verify true} ComputeCoSlice(
+	S: Statement, 
+	V: seq<Variable>, 
+	Vr: seq<Variable>, 
+	fVr: seq<Variable>) 
+returns (Scov: Statement)
+requires Valid(S)
+requires Vr <= V
+requires |Vr| == |fVr|
+requires forall v :: v in V ==> v !in fVr
+requires forall v :: v in glob(S) ==> v !in fVr
+requires forall v :: v in fVr ==> v !in V
+requires forall v :: v in fVr ==> v !in glob(S)
+ensures Valid(Scov)
+ensures forall v :: v in Vr ==> v !in glob(Scov)
+ensures forall v :: v in glob(Scov) ==> v !in Vr
+{
+	var coV := def(S) - setOf(V);
+	var S' := FinalUseSubstitution(S, Vr, fVr);
+	Scov := ComputeSlice(S', coV);
+	assert forall v :: v in Vr ==> v !in glob(Scov) by {
+		assert Vr <= V;
+		assert forall v :: v in coV ==> v !in Vr;
+		assert forall v :: v in Vr ==> v !in coV;
+		assert forall v :: v in Vr ==> v !in glob(S');
+		assert forall v :: v in glob(S') ==> v !in Vr;
+		assert glob(Scov) <= glob(S');
+	}
+}
+
